engine/PrisonersDilemma/Theorems/EBot.lean
@@ -1,0 +1,39 @@
+import PrisonersDilemma.Bots.EBot
+import PrisonersDilemma.Bots.CooperateBot
+import PrisonersDilemma.Bots.DefectBot
+import PrisonersDilemma.Theorems.Helpers
+
+
+open PDNew.Bots
+namespace PDNew.Theorems
+
+theorem EBot_plays_D_against_CooperateBot (fuel : Nat) :
+    play (fuel + 3) EBot CooperateBot = some .D := by
+    apply play_from_eval
+    unfold EBot CooperateBot
+    simp [eval, Prog.subst]
+    intro h
+    have : (Action.C == Action.C) = true := by decide
+    simp [this] at h
+
+theorem EBot_vs_CooperateBot (fuel : Nat):
+    outcome (fuel + 3) EBot CooperateBot = some (.D, .C) := by
+    have hA : play (fuel + 3) EBot CooperateBot = some .D := EBot_plays_D_against_CooperateBot (fuel)
+    have hB : play (fuel + 3) CooperateBot EBot = some .C := rfl
+    simp [outcome, hA, hB]
+
+theorem EBot_plays_D_against_DefectBot (fuel : Nat) :
+    play (fuel + 5) EBot DefectBot = some .D := by
+    apply play_from_eval
+    unfold EBot DefectBot
+    simp [eval, Prog.subst]
+    intro h
+    simp [h]
+
+theorem EBot_vs_DefectBot (fuel : Nat):
+    outcome (fuel + 5) EBot DefectBot = some (.D, .D) := by
+    have hA : play (fuel + 5) EBot DefectBot = some .D := EBot_plays_D_against_DefectBot (fuel)
+    have hB : play (fuel + 5) DefectBot EBot = some .D := rfl
+    simp [outcome, hA, hB]
+
+end PDNew.Theorems
